\section*{Exercise 1.14}

\begin{proof}
We will prove this by induction.
The induction hypothesis $IH(n)$ is that
the result of \texttt{partial-vector-sum} is correct. i.e.:

\[
    \texttt{partial-vector-sum}(v,n) = \sum_{i=0}^{n}v_i
\]

We first show that $IH(0)$ holds. If $n=0$, the result is:

\[
    \texttt{(vector-ref v 0)} = v_0 = \sum_{i=0}^{0}v_i
\]

Therefore, $IH(0)$ holds.

Let $IH(k)$ holds true, we want to show that $IH(k+1)$ holds as well
to complete the induction.

Since $0 \le n < length(v)$, we know that $k + 1 \neq 0$, therefore:

\begin{align*}
    & \texttt{(+ (vector-ref v <k+1>) (partial-vector-sum v (- <k+1> 1)))} \\
    = & v_{k+1} + \texttt{(partial-vector-sum v k)} \\
    = & v_{k+1} + \sum_{i=0}^{k}v_i \\
    = & \sum_{i=0}^{k+1}v_i
\end{align*}

This completes the proof of the claim that $IH(k+1)$ holds and therefore
completes the induction.

\end{proof}
