\section*{Exercise 1.2}

\subsection*{Q1}

As $n$ keeps increasing, we define function $f$:

\begin{equation*}
    f(n) =
    \begin{cases}
        (0,1) & n = 0, \\
        ((n-1)+1, k'+7) & n > 0 \text{ and } f(n-1) = (n-1,k').
    \end{cases}
\end{equation*}

Let $g(n) = cdr(f(n))$, thus:

\begin{align*}
    car(f(n)) & = n \\
    cdr(f(n)) & = g(n) = g(n-1) + 7 (n > 0)
\end{align*}

Therefore, the answer is:

\begin{equation*}
    \{ (n,7n+1) | n \in N \}
\end{equation*}

\subsection*{Q2}

Define $f$ and $g$:

\begin{equation*}
    (f(n), g(n)) =
    \begin{cases}
        (0,1) & n = 0 \\
        ((n'+1, 2k') & n > 0 \text{ and } (f(n-1),g(n-1)) = (n',k')
    \end{cases}
\end{equation*}

For $n > 0$, we have:

\begin{align*}
    f(n) & = f(n-1) + 1 \\
    g(n) & = g(n-1) * 2 
\end{align*}

And we can further conclude that:

\begin{align*}
    f(n) & = n \\
    g(n) & = 2^n 
\end{align*}

Therefore, the answer is:

\begin{equation*}
    \{ (n,2^n) | n \in N \}
\end{equation*}

\subsection*{Q3}

Define $f$, $g$ and $h$:

\begin{equation*}
    (f, g, h)(n) =
    \begin{cases}
        (0,0,1) & n = 0 \\
        ((n'+1, j', i'+j') & n > 0 \text{ and }
            (f,g,h)(n-1) = (n',i',j')
    \end{cases}
\end{equation*}

For $n > 0$, we have:

\begin{align*}
    f(n) & = f(n-1) + 1 \\
    g(n) & = h(n-1) \\
    h(n) & = g(n-1) + h(n-1) = h(n-2) + h(n-1)
\end{align*}

And we can further conclude that:

\begin{align*}
    f(n) & = n \\
    g(n) & = h(n-1) \\
    h(n) & = h(n-2) + h(n-1)
\end{align*}

Let $fib(n)$ denotes the $n^{th}$ Fibonacci number, $fib(0) = 0, fib(1) = 1$.

Therefore, the answer is:

\begin{equation*}
    \{ (n,fib(n),fib(n+1)) | n \in N \}
\end{equation*}

\subsection*{Q4}

Define $f$, $g$ and $h$:

\begin{equation*}
    (f, g, h)(n) =
    \begin{cases}
        (0,1,0) & n = 0 \\
        ((n'+1, i'+2, i'+j') & n > 0 \text{ and }
            (f,g,h)(n-1) = (n',i',j')
    \end{cases}
\end{equation*}

For $n > 0$, we have:

\begin{align*}
    f(n) & = f(n-1) + 1 \\
    g(n) & = g(n-1) + 2 \\
    h(n) & = g(n-1) + h(n-1)
\end{align*}

And we can further conclude that:

\begin{align*}
    f(n) & = n \\
    g(n) & = 2n+1 \\
    h(n) & = \sum_{i=0}^{n-1} g(i) = 1 \cdot n + \frac{(n-1)n}{2} \cdot 2 = n^2
\end{align*}

Therefore, the answer is:

\begin{equation*}
    \{ (n,2n+1,n^2) | n \in N \}
\end{equation*}
