\section*{Exercise 4.17}

Grammar:

\texttt{
    $Expression ::= $ let $\{Identifier$ = $Expression\}^*$ in $Expression$
}

\texttt{
    $Expression ::= $ proc ($\{Identifier\}^{*(,)}$) $Expression$
}

\texttt{
    $Expression ::= $ ($Expression$  $\{Expression\}^{*}$) 
}

\begin{center}
\begin{lstlisting}[mathescape]

; definitions
(define-datatype expression expression?
  ...
  (let-exp
    (vars (list-of identifier?))
    (vals (list-of expression?))
    (body expression?))
  (proc-exp
    (args (list-of identifier?))
    (body expression?))
  
  (call-exp
    (rator expression?)
    (rands (list-of expression?)))
  
  ...)

; assumptions
; $l_i \notin dom(\sigma_{i+1})$
(value-of $exp_0$ $\rho$ $\sigma_0$) = ($val_0$,$\sigma_1$)
(value-of $exp_1$ $\rho$ $\sigma_1$) = ($val_1$,$\sigma_2$)
...
(value-of $exp_n$ $\rho$ $\sigma_n$) = ($val_n$,$\sigma_{n+1}$)

; rules for let-exp:

(value-of (let-exp
            ($var_0$,$var_1$,...,$var_n$)
            ($exp_0$,$exp_1$,...,$exp_n$)
            $body$) $\rho$ $\sigma_0$) =
(value-of
  $body$
  $[var_0=l_0][var_1=l_1]...[var_n=l_n]\rho$
  $[l_0=val_0][l_1=val_1]...[l_n=val_n]\sigma_{n+1}$)

; rules for proc-exp:

(value-of (proc-exp ($var_0$,$var_1$,...,$var_n$) $body$) $\rho$ $\sigma$) =
((proc-val (procedure ($var_0$,$var_1$,...,$var_n$) $body$ $\rho$)), $\sigma$)

; rules for call-exp:
(apply-procedure
  (procedure ($var_0$,$var_1$,...,$var_n$) $body$ $\rho$)
  $val_0$ $val_1$ ... $val_n$ $\sigma_0$) = 
(value-of
  $body$
  $[var_0=l_0][var_1=l_1]...[var_n=l_n]\rho$
  $[l_0=val_0][l_1=val_1]...[l_n=val_n]\sigma_{n+1}$)

\end{lstlisting}
\end{center}
