\documentclass[11pt]{article}

\usepackage{amsmath}

\usepackage{fancyhdr}
\usepackage{amssymb}
\usepackage{amsthm}
\usepackage{xspace}
\usepackage{indentfirst}

\usepackage{diagrams}
\usepackage{mathtools}
\DeclarePairedDelimiter\ceil{\lceil}{\rceil}
\DeclarePairedDelimiter\floor{\lfloor}{\rfloor}

\title{My Exercise Answers to \\
Introduction to Category Theory}
\author{Javran Cheng}

\begin{document}

\maketitle

\newcommand{\cat}[1]{\textit{#1}}
\newcommand{\fcomp}{\circ}

\newcommand{\nat}{\mathbb{N}}

\section{Categories}

\input{exercise-1-1s.tex}
\input{exercise-1-2s.tex}

\subsection{An arrow need not be a function}

\subsubsection{Show that strictly positive integers as objects
and matrices as arrows gives a category}

\begin{itemize}
  \item Objects are strictly positive integers.
  \item Let $m$ and $n$ be two objects, the arrow between them
    ($n \rTo^A m$)
    is an $m \times n$ matrix $A$.
  \item Given two compatible matrices:
    $n \rTo^B k$ and $k \rTo^A m$,
    the arrow composition is given by the matrix product $AB$:
    $n \rTo^{A \fcomp B} m$.
  \item The associativity holds because for any three compatible matrices $A$,$B$ and $C$,
    the matrix multiplication is associative: $(AB)C = A(BC)$.
    Therefore the associativity for arrow composition is obtained from the matrix
    multiplication.
  \item For any object $n$, the identity arrow is the identity matrix $E_n$.
    It holds that $f \fcomp id_n = f = id_m \fcomp f$ for any arrow $f : n \rTo^A m$
    ($A$ is the corresponding matrix of $f$) because of the following property for
    matrix multiplication holds: $ A \times E_n = A = E_m \times A$.
\end{itemize}

Therefore this gives a category. If we have to say that this example somehow cheats,
I think the cheating part is that this category just uses matrix multiplication
to make every property necessary to form a category hold.

\subsubsection{With the appropriate notion of composition,
 graphs and their morphisms form a category}

Suppose we have three directed graphs, namely $(N,E), (M,F), (O,G)$:

\begin{diagram}
  E & \pile{\rTo^{\sigma_0} \\ \rTo_{\tau_0}} & N & \
  F & \pile{\rTo^{\sigma_1} \\ \rTo_{\tau_1}} & M & \
  G & \pile{\rTo^{\sigma_2} \\ \rTo_{\tau_2}} & O & \
\end{diagram}

and two morphisms $f,g$ between them:

\begin{diagram}
  (N,E) & \rTo^f & (M,F) & \rTo^g & (O,G)
\end{diagram}

Graph morphism $f$ consists of two functions $f_0, f_1$, such that:

\begin{align*}
  \sigma_1 \fcomp f_1 = f_0 \fcomp \sigma_0 \qquad \
  \tau_1 \fcomp f_1 = f_0 \fcomp \tau_0
\end{align*}

Similarly, for graph morphism $g$ we have:

\begin{align*}
  \sigma_2 \fcomp g_1 = g_0 \fcomp \sigma_1 \qquad \
  \tau_2 \fcomp f_1 = f_0 \fcomp \tau_1
\end{align*}

Suppose $E_0, F_0, G_0$ are edges in $E,F,G$ respectively
and $N_0 = \sigma_0(E_0), M_0 = \sigma_1(F_0), O_0 = \sigma_2(G_0)$.

We have the following diagram:

\begin{diagram}
  E_0             & \rTo^{f_1} & F_0             & \rTo^{g_1} & G_0 \\
  \dTo^{\sigma_0} &            & \dTo^{\sigma_1} &            & \dTo^{\sigma_2} \\
  N_0             & \rTo^{f_0} & M_0             & \rTo^{g_0} & O_0
\end{diagram}

Since $\sigma_1 \fcomp f_1 = f_0 \fcomp \sigma_0$
and $\sigma_2 \fcomp g_1 = g_0 \fcomp \sigma_1$,
we know that $g_0 \fcomp \sigma_1 \fcomp f_1 = g_0 \fcomp f_0 \fcomp \sigma_0 \
= \sigma_2 \fcomp g_1 \fcomp f_1$.

Similarly, we can conclude that $g_0 \fcomp f_0 \fcomp \tau_0 \
= \tau_2 \fcomp g_1 \fcomp f_1$.

If we denote graph morphisms as pairs of functions, then $f = (f_0,f_1)$ and $g = (g_0,g_1)$.
And we can define the composition of $f$ and $g$ as:

\begin{equation*}
  g \fcomp f = (g_0 \fcomp f_0, g_1 \fcomp f_1)
\end{equation*}

And the composition preserves the property that the following holds:

\begin{align*}
  \sigma_2 \fcomp (g_1 \fcomp f_1) & = (g_0 \fcomp f_0) \fcomp \sigma_0 \\
  \tau_2 \fcomp (g_1 \fcomp f_1) & = (g_0 \fcomp f_0) \fcomp \tau_0
\end{align*}

Therefore we can verify that by taking graphs as objects, graph morphisms as arrows,
and the graph morphism composition defined above as arrow composition, we can form a category.
The associativity of composition holds since:

\begin{align*}
  & (h \fcomp g) \fcomp f \\
  = & ((h_0 \fcomp g_0) \fcomp f_0, (h_1 \fcomp g_1) \fcomp f_1) \\
  = & (h_0 \fcomp (g_0 \fcomp f_0), h_1 \fcomp (g_1 \fcomp f_1)) \\
  = & h \fcomp (g \fcomp f)
\end{align*}

And each identity arrow is the corresponding identity function viewed as graph morphism.

\subsubsection{With the obvious composition this does form a category}

The objects and arrows are given here. So we only need to find a way to compose arrows,
verify its associativity, and find identity arrows.

Consider two new compatible arrows:

\begin{diagram}
  (A,R) & \rTo^{(f,\phi)} & (B,S) & \rTo^{(g,\psi)} & (C,T)
\end{diagram}

where $A,B,C$ are \cat{A}-objects and $R,S,T$ are \cat{S}-objects.

The arrow composition can be defined as:

\begin{align*}
  (g,\psi) \fcomp (f,\phi) = (g \fcomp f, \phi \fcomp \psi)
\end{align*}

We can verify that:

\begin{diagram}
  A & \rTo^{g \fcomp f} & C & R & \lTo^{\phi \fcomp \psi} & T
\end{diagram}

Therefore arrow composition produces another arrow between $(A,R)$ and $(C,T)$.

Given 3 arbitrary compatible arrows $(f,\phi), (g,\psi), (h,\eta)$,
we need to show that the arrow composition is associativity:

\begin{align*}
  & (h,\eta) \fcomp ((g,\psi) \fcomp (f,\phi)) \\
  = & (h,\eta) \fcomp (g \fcomp f, \phi \fcomp \psi) \\
  = & (h \fcomp (g \fcomp f), (\phi \fcomp \psi) \fcomp \eta) \\
  = & ((h \fcomp g) \fcomp f, \phi \fcomp (\psi \fcomp \eta)) \\
  = & (h \fcomp g, \psi \fcomp \eta) \fcomp (f, \phi) \\
  = & ((h,\eta) \fcomp (g,\psi)) \fcomp (f,\phi)
\end{align*}

And each identity arrow is the corresponding pair of identity functions
viewed as a pair of arrows.

\subsubsection{With the obvious composition this does form a category (SetR)}

The arrow composition can be defined in the following way:

For two arbitrary compatible arrows $(f,\phi)$ and $(g,\psi)$, where

\begin{diagram}
  (A,R) & \rTo^{(f,\phi)} & (B,S) & \rTo^{(g,\psi)} & (C,T)
\end{diagram}

The arrow composition is:

\begin{align*}
  (g,\psi) \fcomp (f,\phi) = (g \fcomp f, \phi \fcomp \psi)
\end{align*}

We need to prove that the arrow composition produces an arrow from $(A,R)$ to $(C,T)$,
which has the following property:

\begin{align*}
  \forall a \in A, t \in T, (g \fcomp f)(a (\phi \fcomp \psi)(t)) = \
  (g \fcomp f)(a)t
\end{align*}

\begin{proof}
  The following facts are known:

  \begin{align*}
    \forall a \in A, s \in S, & f(a\phi(s)) = f(a)s \\
    \forall b \in B, t \in T, & g(b\psi(t)) = g(b)t
  \end{align*}

  Since $\psi(t) \in S$, we know that
  $ f(a \phi(\psi(t))) = f(a (\phi \fcomp \psi)(t)) = f(a) \psi(t) $.

  Therefore $\forall a \in A, t \in T$,

  \begin{align*}
    & (g \fcomp f)(a (\phi \fcomp \psi)(t)) \\
    = & g(f(a (\phi \fcomp \psi)(t)) ) \\
    = & g(f(a) \psi(t) ) & f(a) \in B \\
    = & g(f(a))t = (g \fcomp f)(a)t
  \end{align*}

\end{proof}

The associativity of arrow composition holds in the same way that
the arrow composition in exercise $1.3.1$ holds, and each identity arrow
is the corresponding pair of identity functions viewed as an arrow.

Therefore, using the arrow composition described above
gives a category.

% 1.3.5

\subsubsection{}

\begin{proof}
The defined composition is associative.

Consider \cat{RelA}-arrows $F$, $G$ and $H$:

\begin{diagram}
A & \rTo^F & B & \rTo^G & C & \rTo^H & D
\end{diagram}

For $a \in A, d \in D$, consider the composition $d(H \fcomp (G \fcomp F))a$:

\begin{align*}
                & d(H \fcomp (G \fcomp F))a \\
\Leftrightarrow & (\exists c \in C)[dHc(G \fcomp F)a] \\
\Leftrightarrow & (\exists c \in C, \exists b \in B)[dHcGbFa] \\
\Leftrightarrow & (\exists b \in B)[d(H \fcomp G)bFa] \\
\Leftrightarrow & d((H \fcomp G) \fcomp F)a
\end{align*}

Therefore the composition is associate and it does form a category.
\end{proof}

\begin{proof}
For each pair of composible \cat{Set}-arrows $f : A \rTo B$, $g : B \rTo C$:

\[
\forall a \in A, b \in B, b\Gamma(f)a \Leftrightarrow b = f(a)
\]
\[
\forall b \in B, c \in C, c\Gamma(g)b \Leftrightarrow c = g(b)
\]

Therefore, $\forall a \in A, c \in C$:

\begin{align*}
                &  c(\Gamma(g) \fcomp \Gamma(f))a \\
\Leftrightarrow & (\exists b \in B)[c\Gamma(g)b\Gamma(f)a] \\
\Leftrightarrow & (\exists b \in B)[c\Gamma(g)b \wedge b\Gamma(f)a] \\
\Leftrightarrow & (\exists b \in B)[c = g(b) \wedge b = f(a)] \\
\Leftrightarrow & c = g(f(a)) \\
\Leftrightarrow & c = (g \fcomp f)a \\
\Leftrightarrow & c\Gamma(g \fcomp f)a
\end{align*}

Therefore $\Gamma(g \fcomp f) = \Gamma(g) \fcomp \Gamma(f)$

\end{proof}


% 1.3.6
\subsubsection{}

\textbf{(1)}

\begin{proof}
To show that $f \dashv g$, we need to show that
\[
\forall a \in S, b \in T, f(a) \le b \Leftrightarrow a \le g(b)
\]

First we prove that $\forall a \in S, b \in T, f(a) \le b \Rightarrow a \le g(b)$.

From hypothesis we know that $f(a) \le b$ and since $g$ is a monotonic function,
we have $(g \circ f)(a) \le g(b)$.

Because $id_S \le g \circ f$, we know that $a \le (g \circ f)(a)$. Since $S$ is a poset,
$(\le)$ is transitive, we conclude that $a \le g(b)$.

Then we prove that $forall a \in S, b \in T, a \le g(b) \Rightarrow f(a) \le b$.

From hypothesis we have $a \le g(b)$, therefore $f(a) \le (f \circ g)(b)$
because $f$ is a monotonic function.
And we also know that $(f \circ g)(b) \le b$.

We therefore conclude that $f(a) \le b$ because of the transitivity of $(\le)$.

\end{proof}

\textbf{(2)}

\begin{proof}
From $id_S \le g \circ f$, we apply monotonic function $f$ on both side of this inequation:

\[
\forall a \in S, f(a) \le (f \circ g \circ f)(a)
\]

Since we know that

\[
\forall b \in T, (f \circ g)(b) \le b
\]

For a particular case $b = f(a) \in T$, we have:

\[
\forall a \in S, (f \circ g \circ f)(a) \le f(a)
\]

Because $(\le)$ is antisymmetric, we conclude that

\[
\forall a \in S, f(a) = (f \circ g \circ f)(a)
\]

Similarly, from $f \circ g \le id_T$, apply monotonic function $g$ on both side of this inequation:

\[
\forall b \in T, (g \circ f \circ g)(b) \le g(b)
\]

In addition, for a particular $a = g(b) \in S$, we have:

\[
\forall b \in T, g(b) \le (g \circ f \circ g)(b)
\]

Because $(\le)$ is antisymmetric, we conclude that

\[
\forall b \in T, g(b) = (g \circ f \circ g)(b)
\]

\end{proof}


% 1.3.7
\subsubsection{}

\begin{proof}
Suppose we have two \cat{Pos}-arrows $f_1 \dashv g_1$
and $f_2 \dashv g_2$:

\begin{diagram}
A & \rPto^{f_1 \dashv g_1} & B & \rPto^{f_2 \dashv g_2} & C
\end{diagram}

And two arrows can be composed:

\begin{diagram}
A & \rPto^{(f_2 \circ f_1) \dashv (g_1 \circ g_2)} & C
\end{diagram}

Since $(f_1,g_1)$ and $(f_2,g_2)$ are both $\cat{Pos}^{pp}$-arrows,
we have $g_1 \circ f_1 = id_A$ and $g_2 \circ f_2 = id_B$.

For the composed arrow $(f_2 \circ f_1, g_1 \circ g_2)$:

\begin{align*}
  & g \circ f \\
= & g_1 \circ g_2 \circ f_2 \circ f_1 \\
= & g_1 \circ id_B \circ f_1 \\
= & g_1 \circ f_1 \\
= & id_A
\end{align*}

Therefore  $(f_2 \circ f_1, g_1 \circ g_2)$ is also a  $\cat{Pos}^{pp}$-arrow,
projection pairs are closed under composition.

\end{proof}

% 1.3.8

\subsubsection{}

We first prove a lemma: if $f : \mathbb{R} \rTo \mathbb{Z}$, is a monotonic function,
and $\forall z \in \mathbb{Z}, f(z) = z$, then $f$ can only be one of the following functions:

\begin{itemize}
\item $f(x) = \floor{x}$
\item $f(x) = \ceil{x}$
\end{itemize}

\begin{proof}
For any given $r \in \mathbb{R}, r \notin \mathbb{Z}$, there exists a $z \in \mathbb{Z}$ such that
$z \le r \le z+1$. Since $f$ is a monotone, we know that $f(z) = z \le f(r) \le f(z+1) = z+1$.

Because $\forall r \in \mathbb{R}, f(r) \in \mathbb{Z}$, we know
$\forall r \in \mathbb{R}, f(r) \in \{\floor{r}, \ceil{r}\}$

Suppose $\exists r \in \mathbb{R}, f(r) = \floor{r}$, then $\forall r_1 \in \mathbb{R}$,
if $r_1 \le r$, then we must have $f(r_1) \le f(r) = \floor{r}$. This conclusion implies that
if $\exists r \in \mathbb{R}, f(r) = \floor{r}$, then $\forall r \in \mathbb{R}, f(r) = \floor{r}$

Similarly, we have the conclusion that if $\exists r \in \mathbb{R}, f(r) = \ceil{r}$, then $\forall r \in \mathbb{R}, f(r) = \ceil{r}$

Therefore either $\forall r \in \mathbb{R}, f(r) = \floor{r}$ holds, or $\forall r \in \mathbb{R}, f(r) = \ceil{r}$ holds.

\end{proof}

\textbf{(a)} Consider $\iota \dashv \rho$, $\forall z \in \mathbb{Z}, r \in \mathbb{R}$, we have:

\[
\iota(z)=z \le r \Leftrightarrow z \le \rho(r)
\]

Notice that when $r \in \mathbb{Z}$, we have $\rho(r) = r$. We can apply the previous lemma
and conclude that $\rho$ is either the floor function, or the ceiling function. But the property that
$\iota(z) \le r \Leftrightarrow z \le \rho(r)$ only holds when $\rho$ is the floor function.

Therefore we conclude that $\forall r \in \mathbb{R}, f(r) = \floor{r}$.

Similarly, consider $\lambda \dashv \iota$, $\forall z \in \mathbb{Z}, r \in \mathbb{R}$, we have:

\[
\lambda(r) \le z \Leftrightarrow r \le \iota(z) = z
\]

Since when $r \in \mathbb{Z},\lambda(r) = r$. Apply the previous lemma, we conclude that $\lambda$ is either the floor function, or the ceiling function. But the property that
$\lambda(r) \le z \Leftrightarrow r \le \iota(z)$ only holds when $\lambda$ is the ceiling function.

Therefore we have proved the uniqueness of $\rho$ and $\lambda$, such that

\begin{diagram}
\mathbb{Z} & \rPto^{\iota \dashv \rho} & \mathbb{R} & \rPto^{\lambda \dashv \iota} & \mathbb{Z}
\end{diagram}

\textbf{(b)} $(\lambda \dashv \iota) \fcomp (\iota \dashv \rho) = (\lambda \fcomp \iota \dashv \rho \fcomp \iota)$

The arrow composition result is $f \dashv g$, in which $f = \lambda \fcomp \iota, g = \rho \fcomp \iota$.

\begin{align*}
g \fcomp f & = \rho \fcomp \iota \fcomp \lambda \fcomp \iota \\
           & = \rho \fcomp \lambda \\
           & = \lambda
\end{align*}

Since $\forall z \in \mathbb{Z}, \lambda(z) = \ceil{z} = z$, we can conclude that $g \fcomp f = id_\mathbb{Z}$.

Also that:

\begin{align*}
f \fcomp g & = \lambda \fcomp \iota \fcomp \rho \fcomp \iota \\
	       & = \lambda \fcomp \rho \\
	       & = \rho
\end{align*}

Notice that $\forall r \in \mathbb{R}, \rho(\rho(r)) = \rho(\floor{r}) = \rho(r)$,
we conclude the other composition $f \fcomp g = \rho$ is idempotent.

\textbf{(c)} For $\iota \dashv \rho$, $\rho \fcomp \iota = \rho$.
Since $\forall z \in \mathbb{Z}, \rho(z) = z$, we can conclude $\rho \fcomp \iota = \rho = id_\mathbb{Z}$.

Thus $\iota \dashv \rho$ is a $\cat{Pos}^{pp}$-arrow.

However, for $\lambda \dashv \iota$, $\iota \fcomp \lambda = \lambda$. $\exists r \in \mathbb{R}, \lambda(r) \neq r$.

Therefore $\lambda \dashv \iota$ is not a $\cat{Pos}^{pp}$-arrow.

\end{document}
